Arrays, revisited. Now require a serializer.

src/lowparse/LowParse.SLow.Array.fst
@@ -1,58 +1,38 @@
 module LowParse.SLow.Array
 include LowParse.SLow.FLData
+include LowParse.SLow.VLData
 include LowParse.SLow.List
 include LowParse.Spec.Array
 
 module U32 = FStar.UInt32
-
-#set-options "--z3rlimit 32"
-
-inline_for_extraction
-let parse32_array'
-  (#k: parser_kind)
-  (#t: Type0)
-  (#p: parser k t)
-  (p32: parser32 p)
-  (array_byte_size: nat)
-  (array_byte_size32: U32.t { U32.v array_byte_size32 == array_byte_size } )
-  (precond: unit { array_type_of_parser_kind_precond p array_byte_size == true } )
-: Tot (parser32 (parse_array' p array_byte_size precond))
-= assert_norm (array_type_of_parser p array_byte_size == (x: list t { array_pred (array_byte_size / k.parser_kind_low) x}));
-  coerce_parser32
-    (array_type_of_parser p array_byte_size)
-    (parse32_strengthen
-          #_
-          #_
-          #(parse_fldata (parse_list p) array_byte_size)
-          (parse32_fldata (parse32_list p32) array_byte_size array_byte_size32)
-          (array_pred (array_byte_size / k.parser_kind_low))
-          (parse_array_correct p array_byte_size precond)
-    )
-    ()
 
 inline_for_extraction
 let parse32_array
   (#k: parser_kind)
   (#t: Type0)
   (#p: parser k t)
+  (s: serializer p)
   (p32: parser32 p)
   (array_byte_size: nat)
   (array_byte_size32: U32.t { U32.v array_byte_size32 == array_byte_size } )
-  (precond: unit { array_type_of_parser_kind_precond p array_byte_size == true } )
-: Tot (parser32 (parse_array p array_byte_size precond))
-= make_parser32
-    (parse_array p array_byte_size precond)
-    (fun (input: bytes32) ->
-      let res = // : option ((l: list t { array_pred (array_byte_size / k.parser_kind_low) l } ) * U32.t) =
-        parse32_array' p32 array_byte_size array_byte_size32 precond
-          input
-      in
-      match res with
-      | None -> None
-      | Some (x, consumed) ->
-        let x1 : list t = x in
-        Some ((x1 <: array_type_of_parser p array_byte_size), consumed)
+  (elem_count: nat)
+  (u : unit { fldata_array_precond p array_byte_size elem_count == true } )
+: Tot (parser32 (parse_array s array_byte_size elem_count))
+= [@inline_let]
+  let _ =
+    fldata_to_array_inj s array_byte_size elem_count u
+  in
+  parse32_synth
+    _
+    (fldata_to_array s array_byte_size elem_count u)
+    (fun x -> fldata_to_array s array_byte_size elem_count u x)
+    (parse32_fldata_strong
+      (serialize_list _ s)
+      (parse32_list p32)
+      array_byte_size
+      array_byte_size32
     )
+    ()
 
 inline_for_extraction
 let serialize32_array
@@ -60,51 +40,98 @@ let serialize32_array
   (#t: Type0)
   (#p: parser k t)
   (#s: serializer p)
-  (s32: serializer32 s)
+  (s32: partial_serializer32 s)
   (array_byte_size: nat { array_byte_size < 4294967296 } )
-  (precond: unit { array_type_of_parser_kind_precond p array_byte_size == true } )
-  (lprecond: unit { serialize_list_precond k } )
-: Tot (serializer32 (serialize_array s array_byte_size precond lprecond))
-= fun (input: array_type_of_parser p array_byte_size) ->
-  serialize32_fldata_strong (partial_serialize32_list _ _ s32 lprecond) array_byte_size (synth_array_recip s array_byte_size precond lprecond input)
-  <: (res: bytes32 { serializer32_correct (serialize_array s array_byte_size precond lprecond) input res })
-
-include LowParse.SLow.VLData
+  (elem_count: nat)
+  (u : unit { fldata_array_precond p array_byte_size elem_count == true } )
+: Tot (serializer32 (serialize_array s array_byte_size elem_count u))
+= [@inline_let]
+  let _ =
+    fldata_to_array_inj s array_byte_size elem_count u
+  in
+  [@inline_let]
+  let _ =
+    array_to_fldata_to_array s array_byte_size elem_count u
+  in
+  serialize32_synth
+    _
+    (fldata_to_array s array_byte_size elem_count u)
+    _
+    (serialize32_fldata_strong
+      (partial_serialize32_list _ _ s32 ())
+      array_byte_size
+    )
+    (array_to_fldata s array_byte_size elem_count u)
+    (fun x -> array_to_fldata s array_byte_size elem_count u x)
+    ()
 
 inline_for_extraction
 let parse32_vlarray
-  (#k: parser_kind)
-  (#t: Type0)
-  (#p: parser k t)
-  (p32: parser32 p)
   (array_byte_size_min: nat)
   (array_byte_size_min32: U32.t { U32.v array_byte_size_min32 == array_byte_size_min } )
   (array_byte_size_max: nat)
-  (array_byte_size_max32: U32.t { U32.v array_byte_size_max32 == array_byte_size_max } )  
-  (precond: unit {vlarray_type_of_parser_kind_precond p array_byte_size_min array_byte_size_max == true})
-: Tot (parser32 (parse_vlarray p array_byte_size_min array_byte_size_max precond))
-= let elem_byte_size : pos = k.parser_kind_low in
-  parse32_strengthen
-    (parse32_bounded_vldata
+  (array_byte_size_max32: U32.t { U32.v array_byte_size_max32 == array_byte_size_max } )
+  (#k: parser_kind)
+  (#t: Type0)
+  (#p: parser k t)
+  (s: serializer p)
+  (p32: parser32 p)
+  (elem_count_min: nat)
+  (elem_count_max: nat)
+  (u: unit {
+    vldata_vlarray_precond array_byte_size_min array_byte_size_max p elem_count_min elem_count_max == true  
+  })
+: Tot (parser32 (parse_vlarray array_byte_size_min array_byte_size_max s elem_count_min elem_count_max u))
+= [@inline_let]
+  let _ =
+    vldata_to_vlarray_inj array_byte_size_min array_byte_size_max s elem_count_min elem_count_max u
+  in
+  parse32_synth
+    _
+    (vldata_to_vlarray array_byte_size_min array_byte_size_max s elem_count_min elem_count_max u)
+    (fun x -> vldata_to_vlarray array_byte_size_min array_byte_size_max s elem_count_min elem_count_max u x)
+    (parse32_bounded_vldata_strong
       array_byte_size_min
       array_byte_size_min32
       array_byte_size_max
       array_byte_size_max32
+      (serialize_list _ s)
       (parse32_list p32)
     )
-    (vlarray_pred (array_byte_size_min / elem_byte_size) (array_byte_size_max / elem_byte_size))
-    (parse_vlarray_correct p array_byte_size_min array_byte_size_max precond)
+    ()
 
-assume
-val serialize32_bounded_vldata_strong
-  (min: nat)
-  (max: nat { min <= max /\ max > 0 /\ max < 4294967292 } ) // NOTE here: max must be less than 2^32 - 4
+inline_for_extraction
+let serialize32_vlarray
+  (array_byte_size_min: nat)
+  (array_byte_size_max: nat { array_byte_size_max < 4294967292 } ) // NOTE here: max must be less than 2^32 - 4 to account for the size of the length header
   (#k: parser_kind)
   (#t: Type0)
   (#p: parser k t)
   (#s: serializer p)
   (s32: partial_serializer32 s)
-  (array_byte_size_min array_byte_size_max: nat)
-  (precond: unit {vlarray_type_of_parser_kind_precond p array_byte_size_min array_byte_size_max == true})
-  (lprecond: unit { serialize_list_precond k } )
-: Tot (serializer32 (serialize_bounded_vldata_strong min max s))
+  (elem_count_min: nat)
+  (elem_count_max: nat)
+  (u: unit {
+    vldata_vlarray_precond array_byte_size_min array_byte_size_max p elem_count_min elem_count_max == true  
+  })
+: Tot (serializer32 (serialize_vlarray array_byte_size_min array_byte_size_max s elem_count_min elem_count_max u))
+= [@inline_let]
+  let _ =
+    vldata_to_vlarray_inj array_byte_size_min array_byte_size_max s elem_count_min elem_count_max u
+  in
+  [@inline_let]
+  let _ =
+    vlarray_to_vldata_to_vlarray array_byte_size_min array_byte_size_max s elem_count_min elem_count_max u
+  in
+  serialize32_synth
+    _
+    (vldata_to_vlarray array_byte_size_min array_byte_size_max s elem_count_min elem_count_max u)
+    _
+    (serialize32_bounded_vldata_strong
+      array_byte_size_min
+      array_byte_size_max
+      (partial_serialize32_list _ _ s32 ())
+    )
+    (vlarray_to_vldata array_byte_size_min array_byte_size_max s elem_count_min elem_count_max u)
+    (fun x -> vlarray_to_vldata array_byte_size_min array_byte_size_max s elem_count_min elem_count_max u x)
+    ()
